---
title: "Tema 1 - Ejercicio 2"
author: "Curso Álgebra Lineal"
output: pdf_document
---

```{r setup, include=FALSE}
knitr::opts_chunk$set(echo = TRUE, comment = NA)
```

## Enunciado

Dada la matriz $$A = \begin{pmatrix}2&3&-1&2\\3&2&5&0\\-1&7&0&4\\-4&1&-3&7\end{pmatrix}$$ comprobar que se cumple $A+(-A) = (-A)+A=O$

### Solución

Sabemos que $$-A = \begin{pmatrix}-2&-3&1&-2\\-3&-2&-5&0\\1&-7&0&-4\\4&-1&3&-7\end{pmatrix}$$

con lo cual, $$A+(-A) = \begin{pmatrix}2+(-2)&3+(-3)&-1+1&2+(-2)\\3+(-3)&2+(-2)&5+(-5)&0+0\\-1+1&7+(-7)&0+0&4+(-4)\\-4+4&1+(-1)&-3+3&7+(-7)\end{pmatrix} = \begin{pmatrix}0&0&0&0\\0&0&0&0\\0&0&0&0\\0&0&0&0\end{pmatrix} = O$$

y, por otro lado tenemos 

$$(-A)+ A = \begin{pmatrix}-2+2&-3+3&1+(-1)&-2+2\\-3+3&-2+2&-5+5&0+0\\1+(-1)&-7+7&0+0&-4+4\\4+(-4)&-1+1&3+(-3)&-7+7\end{pmatrix} = \begin{pmatrix}0&0&0&0\\0&0&0&0\\0&0&0&0\\0&0&0&0\end{pmatrix} = O$$